# baseURI: https://spec.edmcouncil.org/fibo/ontology/master/2023Q2/LOAN/LoansSpecific/CardAccounts/
# imports: https://spec.edmcouncil.org/fibo/ontology/master/2023Q2/FBC/DebtAndEquities/Debt/
# imports: https://spec.edmcouncil.org/fibo/ontology/master/2023Q2/FBC/FinancialInstruments/FinancialInstruments/
# imports: https://spec.edmcouncil.org/fibo/ontology/master/2023Q2/FBC/ProductsAndServices/ClientsAndAccounts/
# imports: https://spec.edmcouncil.org/fibo/ontology/master/2023Q2/FBC/ProductsAndServices/FinancialProductsAndServices/
# imports: https://spec.edmcouncil.org/fibo/ontology/master/2023Q2/FND/Accounting/CurrencyAmount/
# imports: https://spec.edmcouncil.org/fibo/ontology/master/2023Q2/FND/Agreements/Contracts/
# imports: https://spec.edmcouncil.org/fibo/ontology/master/2023Q2/FND/Arrangements/Documents/
# imports: https://spec.edmcouncil.org/fibo/ontology/master/2023Q2/FND/OwnershipAndControl/Ownership/
# imports: https://spec.edmcouncil.org/fibo/ontology/master/2023Q2/FND/Parties/Parties/
# imports: https://spec.edmcouncil.org/fibo/ontology/master/2023Q2/FND/Parties/Roles/
# imports: https://spec.edmcouncil.org/fibo/ontology/master/2023Q2/FND/Places/Locations/
# imports: https://spec.edmcouncil.org/fibo/ontology/master/2023Q2/FND/Relations/Relations/
# imports: https://spec.edmcouncil.org/fibo/ontology/master/2023Q2/FND/Utilities/AnnotationVocabulary/
# imports: https://www.omg.org/spec/Commons/AnnotationVocabulary/
# imports: https://www.omg.org/spec/Commons/Classifiers/
# imports: https://www.omg.org/spec/Commons/CodesAndCodeSets/
# imports: https://www.omg.org/spec/Commons/ContextualDesignators/
# imports: https://www.omg.org/spec/Commons/DatesAndTimes/
# imports: https://www.omg.org/spec/Commons/Designators/
# imports: https://www.omg.org/spec/Commons/Identifiers/
# imports: https://www.omg.org/spec/LCC/Countries/CountryRepresentation/

@base <https://spec.edmcouncil.org/fibo/ontology/master/2023Q2/LOAN/LoansSpecific/CardAccounts/> .
@prefix cmns-av: <https://www.omg.org/spec/Commons/AnnotationVocabulary/> .
@prefix cmns-cds: <https://www.omg.org/spec/Commons/CodesAndCodeSets/> .
@prefix cmns-cls: <https://www.omg.org/spec/Commons/Classifiers/> .
@prefix cmns-cxtdsg: <https://www.omg.org/spec/Commons/ContextualDesignators/> .
@prefix cmns-dsg: <https://www.omg.org/spec/Commons/Designators/> .
@prefix cmns-dt: <https://www.omg.org/spec/Commons/DatesAndTimes/> .
@prefix cmns-id: <https://www.omg.org/spec/Commons/Identifiers/> .
@prefix dcterms: <http://purl.org/dc/terms/> .
@prefix fibo-fbc-dae-dbt: <https://spec.edmcouncil.org/fibo/ontology/FBC/DebtAndEquities/Debt/> .
@prefix fibo-fbc-fi-fi: <https://spec.edmcouncil.org/fibo/ontology/FBC/FinancialInstruments/FinancialInstruments/> .
@prefix fibo-fbc-pas-caa: <https://spec.edmcouncil.org/fibo/ontology/FBC/ProductsAndServices/ClientsAndAccounts/> .
@prefix fibo-fbc-pas-fpas: <https://spec.edmcouncil.org/fibo/ontology/FBC/ProductsAndServices/FinancialProductsAndServices/> .
@prefix fibo-fnd-acc-cur: <https://spec.edmcouncil.org/fibo/ontology/FND/Accounting/CurrencyAmount/> .
@prefix fibo-fnd-agr-ctr: <https://spec.edmcouncil.org/fibo/ontology/FND/Agreements/Contracts/> .
@prefix fibo-fnd-arr-doc: <https://spec.edmcouncil.org/fibo/ontology/FND/Arrangements/Documents/> .
@prefix fibo-fnd-oac-own: <https://spec.edmcouncil.org/fibo/ontology/FND/OwnershipAndControl/Ownership/> .
@prefix fibo-fnd-plc-loc: <https://spec.edmcouncil.org/fibo/ontology/FND/Places/Locations/> .
@prefix fibo-fnd-pty-pty: <https://spec.edmcouncil.org/fibo/ontology/FND/Parties/Parties/> .
@prefix fibo-fnd-pty-rl: <https://spec.edmcouncil.org/fibo/ontology/FND/Parties/Roles/> .
@prefix fibo-fnd-rel-rel: <https://spec.edmcouncil.org/fibo/ontology/FND/Relations/Relations/> .
@prefix fibo-fnd-utl-av: <https://spec.edmcouncil.org/fibo/ontology/FND/Utilities/AnnotationVocabulary/> .
@prefix fibo-loan-spc-crd: <https://spec.edmcouncil.org/fibo/ontology/LOAN/LoansSpecific/CardAccounts/> .
@prefix lcc-cr: <https://www.omg.org/spec/LCC/Countries/CountryRepresentation/> .
@prefix owl: <http://www.w3.org/2002/07/owl#> .
@prefix rdf: <http://www.w3.org/1999/02/22-rdf-syntax-ns#> .
@prefix rdfs: <http://www.w3.org/2000/01/rdf-schema#> .
@prefix skos: <http://www.w3.org/2004/02/skos/core#> .
@prefix xsd: <http://www.w3.org/2001/XMLSchema#> .

<https://spec.edmcouncil.org/fibo/ontology/LOAN/LoansSpecific/CardAccounts/>
	a owl:Ontology ;
	rdfs:label "Card Accounts Ontology" ;
	dcterms:abstract "This ontology defines revolving credit account-related concepts that are specific to credit and debit cards. Note that it does not differentiate between consumer and commercial/corporate cards and is capable of representing either." ;
	dcterms:license "https://opensource.org/licenses/MIT"^^xsd:anyURI ;
	owl:imports
		<https://spec.edmcouncil.org/fibo/ontology/master/2023Q2/FBC/DebtAndEquities/Debt/> ,
		<https://spec.edmcouncil.org/fibo/ontology/master/2023Q2/FBC/FinancialInstruments/FinancialInstruments/> ,
		<https://spec.edmcouncil.org/fibo/ontology/master/2023Q2/FBC/ProductsAndServices/ClientsAndAccounts/> ,
		<https://spec.edmcouncil.org/fibo/ontology/master/2023Q2/FBC/ProductsAndServices/FinancialProductsAndServices/> ,
		<https://spec.edmcouncil.org/fibo/ontology/master/2023Q2/FND/Accounting/CurrencyAmount/> ,
		<https://spec.edmcouncil.org/fibo/ontology/master/2023Q2/FND/Agreements/Contracts/> ,
		<https://spec.edmcouncil.org/fibo/ontology/master/2023Q2/FND/Arrangements/Documents/> ,
		<https://spec.edmcouncil.org/fibo/ontology/master/2023Q2/FND/OwnershipAndControl/Ownership/> ,
		<https://spec.edmcouncil.org/fibo/ontology/master/2023Q2/FND/Parties/Parties/> ,
		<https://spec.edmcouncil.org/fibo/ontology/master/2023Q2/FND/Parties/Roles/> ,
		<https://spec.edmcouncil.org/fibo/ontology/master/2023Q2/FND/Places/Locations/> ,
		<https://spec.edmcouncil.org/fibo/ontology/master/2023Q2/FND/Relations/Relations/> ,
		<https://spec.edmcouncil.org/fibo/ontology/master/2023Q2/FND/Utilities/AnnotationVocabulary/> ,
		<https://www.omg.org/spec/Commons/AnnotationVocabulary/> ,
		<https://www.omg.org/spec/Commons/Classifiers/> ,
		<https://www.omg.org/spec/Commons/CodesAndCodeSets/> ,
		<https://www.omg.org/spec/Commons/ContextualDesignators/> ,
		<https://www.omg.org/spec/Commons/DatesAndTimes/> ,
		<https://www.omg.org/spec/Commons/Designators/> ,
		<https://www.omg.org/spec/Commons/Identifiers/> ,
		<https://www.omg.org/spec/LCC/Countries/CountryRepresentation/>
		;
	owl:versionIRI <https://spec.edmcouncil.org/fibo/ontology/master/2023Q2/LOAN/LoansSpecific/CardAccounts/> ;
	fibo-fnd-utl-av:hasMaturityLevel fibo-fnd-utl-av:Release ;
	cmns-av:copyright
		"Copyright (c) 2020-2023 EDM Council, Inc." ,
		"Copyright (c) 2020-2023 Object Management Group, Inc."
		;
	.

fibo-loan-spc-crd:AmericanExpressNetwork
	a
		owl:NamedIndividual ,
		fibo-loan-spc-crd:CreditCardNetwork
		;
	rdfs:label "American Express network" ;
	rdfs:isDefinedBy <https://spec.edmcouncil.org/fibo/ontology/LOAN/LoansSpecific/CardAccounts/> ;
	skos:definition "credit card network and card issuer that both issues credit cards and processes payments for cards bearing its logo, as well as offering cardholder benefits like travel insurance" ;
	.

fibo-loan-spc-crd:CardAccount
	a owl:Class ;
	rdfs:subClassOf
		fibo-fbc-pas-caa:CustomerAccount ,
		[
			a owl:Restriction ;
			owl:onProperty fibo-fbc-pas-caa:isLinkedToAccount ;
			owl:onClass fibo-fbc-pas-caa:CustomerAccount ;
			owl:minQualifiedCardinality "0"^^xsd:nonNegativeInteger ;
		] ,
		[
			a owl:Restriction ;
			owl:onProperty fibo-fbc-pas-caa:hasPrimaryAccountHolder ;
			owl:someValuesFrom fibo-loan-spc-crd:Cardholder ;
		] ,
		[
			a owl:Restriction ;
			owl:onProperty fibo-fbc-pas-caa:realizes ;
			owl:someValuesFrom fibo-loan-spc-crd:CardProduct ;
		] ,
		[
			a owl:Restriction ;
			owl:onProperty cmns-dsg:isDefinedIn ;
			owl:someValuesFrom fibo-loan-spc-crd:PaymentCardAgreement ;
		] ,
		[
			a owl:Restriction ;
			owl:onProperty cmns-dsg:isSignifiedBy ;
			owl:someValuesFrom fibo-loan-spc-crd:PaymentCard ;
		] ,
		[
			a owl:Restriction ;
			owl:onProperty cmns-id:isIdentifiedBy ;
			owl:someValuesFrom fibo-loan-spc-crd:PrimaryCardAccountNumber ;
		]
		;
	rdfs:label "card account" ;
	rdfs:isDefinedBy <https://spec.edmcouncil.org/fibo/ontology/LOAN/LoansSpecific/CardAccounts/> ;
	skos:definition "account whose terms and conditions are defined in a card agreement that is represented by a payment card" ;
	.

fibo-loan-spc-crd:CardAuthenticationValue
	a owl:Class ;
	rdfs:subClassOf fibo-loan-spc-crd:MagneticStripeVerificationCodeValue ;
	rdfs:label "card authentication value" ;
	rdfs:isDefinedBy <https://spec.edmcouncil.org/fibo/ontology/LOAN/LoansSpecific/CardAccounts/> ;
	skos:definition "card verification value specifically for JCB payment cards" ;
	cmns-av:abbreviation "CAV" ;
	cmns-av:adaptedFrom "https://www.pcisecuritystandards.org/pci_security/glossary"^^xsd:anyURI ;
	.

fibo-loan-spc-crd:CardAuthenticationValue2
	a owl:Class ;
	rdfs:subClassOf fibo-loan-spc-crd:ThreeDigitVerificationCodeValue ;
	rdfs:label "card authentication value 2" ;
	rdfs:isDefinedBy <https://spec.edmcouncil.org/fibo/ontology/LOAN/LoansSpecific/CardAccounts/> ;
	skos:definition "card verification value specifically for JCB payment cards" ;
	cmns-av:adaptedFrom "https://www.pcisecuritystandards.org/pci_security/glossary"^^xsd:anyURI ;
	cmns-av:synonym "CAV2" ;
	.

fibo-loan-spc-crd:CardExpirationDate
	a owl:Class ;
	rdfs:subClassOf cmns-dt:ExplicitDate ;
	rdfs:label "card expiration date" ;
	rdfs:isDefinedBy <https://spec.edmcouncil.org/fibo/ontology/LOAN/LoansSpecific/CardAccounts/> ;
	skos:definition "date on which a given payment card expires" ;
	.

fibo-loan-spc-crd:CardIdentificationNumber
	a owl:Class ;
	rdfs:subClassOf fibo-loan-spc-crd:ThreeDigitVerificationCodeValue ;
	rdfs:label "card identification number" ;
	rdfs:isDefinedBy <https://spec.edmcouncil.org/fibo/ontology/LOAN/LoansSpecific/CardAccounts/> ;
	skos:definition "card verification value specifically for American Express and Discover payment cards" ;
	cmns-av:abbreviation "CID" ;
	cmns-av:adaptedFrom "https://www.pcisecuritystandards.org/pci_security/glossary"^^xsd:anyURI ;
	.

fibo-loan-spc-crd:CardProduct
	a owl:Class ;
	rdfs:subClassOf
		fibo-fbc-pas-fpas:FinancialProduct ,
		[
			a owl:Restriction ;
			owl:onProperty fibo-loan-spc-crd:hasCreditCardNetwork ;
			owl:onClass fibo-loan-spc-crd:CreditCardNetwork ;
			owl:minQualifiedCardinality "0"^^xsd:nonNegativeInteger ;
		] ,
		[
			a owl:Restriction ;
			owl:onProperty fibo-fnd-plc-loc:hasSubdivision ;
			owl:onClass lcc-cr:CountrySubdivision ;
			owl:minQualifiedCardinality "0"^^xsd:nonNegativeInteger ;
		] ,
		[
			a owl:Restriction ;
			owl:onProperty fibo-loan-spc-crd:usesCurrency ;
			owl:onClass fibo-fnd-acc-cur:Currency ;
			owl:qualifiedCardinality "1"^^xsd:nonNegativeInteger ;
		] ,
		[
			a owl:Restriction ;
			owl:onProperty fibo-fnd-plc-loc:hasCountry ;
			owl:onClass lcc-cr:Country ;
			owl:qualifiedCardinality "1"^^xsd:nonNegativeInteger ;
		] ,
		[
			a owl:Restriction ;
			owl:onProperty fibo-fbc-pas-caa:isRealizedBy ;
			owl:someValuesFrom fibo-loan-spc-crd:CardAccount ;
		]
		;
	rdfs:label "card product" ;
	rdfs:isDefinedBy <https://spec.edmcouncil.org/fibo/ontology/LOAN/LoansSpecific/CardAccounts/> ;
	skos:definition "financial product involving the issuance of credit, debit, or other payment cards" ;
	.

fibo-loan-spc-crd:CardSecurityCode
	a owl:Class ;
	rdfs:subClassOf fibo-loan-spc-crd:MagneticStripeVerificationCodeValue ;
	rdfs:label "card security code" ;
	rdfs:isDefinedBy <https://spec.edmcouncil.org/fibo/ontology/LOAN/LoansSpecific/CardAccounts/> ;
	skos:definition "card verification value specifically for American Express payment cards" ;
	cmns-av:abbreviation "CSC" ;
	cmns-av:adaptedFrom "https://www.pcisecuritystandards.org/pci_security/glossary"^^xsd:anyURI ;
	.

fibo-loan-spc-crd:CardValidationCode
	a owl:Class ;
	rdfs:subClassOf fibo-loan-spc-crd:MagneticStripeVerificationCodeValue ;
	rdfs:label "card validation code" ;
	rdfs:isDefinedBy <https://spec.edmcouncil.org/fibo/ontology/LOAN/LoansSpecific/CardAccounts/> ;
	skos:definition "card verification code specifically for Mastercard payment cards" ;
	cmns-av:abbreviation "PAN CVC" ;
	cmns-av:adaptedFrom "https://www.pcisecuritystandards.org/pci_security/glossary"^^xsd:anyURI ;
	.

fibo-loan-spc-crd:CardValidationCode2
	a owl:Class ;
	rdfs:subClassOf fibo-loan-spc-crd:ThreeDigitVerificationCodeValue ;
	rdfs:label "card validation code 2" ;
	rdfs:isDefinedBy <https://spec.edmcouncil.org/fibo/ontology/LOAN/LoansSpecific/CardAccounts/> ;
	skos:definition "card verification value specifically for Mastercard payment cards" ;
	cmns-av:abbreviation "PAN CVC2" ;
	cmns-av:adaptedFrom "https://www.pcisecuritystandards.org/pci_security/glossary"^^xsd:anyURI ;
	.

fibo-loan-spc-crd:CardVerificationCodeValue
	a owl:Class ;
	rdfs:subClassOf
		cmns-cds:CodeElement ,
		[
			a owl:Restriction ;
			owl:onProperty fibo-fnd-rel-rel:hasTag ;
			owl:onDataRange xsd:string ;
			owl:qualifiedCardinality "1"^^xsd:nonNegativeInteger ;
		] ,
		[
			a owl:Restriction ;
			owl:onProperty cmns-cxtdsg:appliesTo ;
			owl:someValuesFrom fibo-loan-spc-crd:PaymentCard ;
		]
		;
	rdfs:label "card verification code or value" ;
	rdfs:isDefinedBy <https://spec.edmcouncil.org/fibo/ontology/LOAN/LoansSpecific/CardAccounts/> ;
	skos:definition "code that specifies either (1) magnetic-stripe data, or (2) printed security features that are used to protect data integrity and limit alteration, counterfeiting and fraud generally" ;
	cmns-av:adaptedFrom "https://www.pcisecuritystandards.org/pci_security/glossary"^^xsd:anyURI ;
	.

fibo-loan-spc-crd:CardVerificationValue
	a owl:Class ;
	rdfs:subClassOf fibo-loan-spc-crd:MagneticStripeVerificationCodeValue ;
	rdfs:label "card verification value" ;
	rdfs:isDefinedBy <https://spec.edmcouncil.org/fibo/ontology/LOAN/LoansSpecific/CardAccounts/> ;
	skos:definition "card verification value specifically for Visa and Discover payment cards" ;
	cmns-av:abbreviation "CVV" ;
	cmns-av:adaptedFrom "https://www.pcisecuritystandards.org/pci_security/glossary"^^xsd:anyURI ;
	.

fibo-loan-spc-crd:CardVerificationValue2
	a owl:Class ;
	rdfs:subClassOf fibo-loan-spc-crd:ThreeDigitVerificationCodeValue ;
	rdfs:label "card verification value 2" ;
	rdfs:isDefinedBy <https://spec.edmcouncil.org/fibo/ontology/LOAN/LoansSpecific/CardAccounts/> ;
	skos:definition "card verification value specifically for Visa payment cards" ;
	cmns-av:adaptedFrom "https://www.pcisecuritystandards.org/pci_security/glossary"^^xsd:anyURI ;
	cmns-av:synonym "CVV2" ;
	.

fibo-loan-spc-crd:Cardholder
	a owl:Class ;
	rdfs:subClassOf
		fibo-fbc-pas-caa:CustomerAccountHolder ,
		[
			a owl:Restriction ;
			owl:onProperty fibo-fnd-pty-rl:isPlayedBy ;
			owl:someValuesFrom [
				a owl:Restriction ;
				owl:onProperty fibo-fnd-oac-own:owns ;
				owl:someValuesFrom fibo-loan-spc-crd:CardAccount ;
			] ;
		] ,
		[
			a owl:Restriction ;
			owl:onProperty fibo-fnd-pty-rl:isPlayedBy ;
			owl:someValuesFrom [
				a owl:Restriction ;
				owl:onProperty fibo-fnd-pty-pty:isAPartyTo ;
				owl:someValuesFrom fibo-loan-spc-crd:CardAccount ;
			] ;
		] ,
		[
			a owl:Restriction ;
			owl:onProperty fibo-fnd-rel-rel:holds ;
			owl:someValuesFrom fibo-loan-spc-crd:CardAccount ;
		]
		;
	rdfs:label "cardholder" ;
	rdfs:isDefinedBy <https://spec.edmcouncil.org/fibo/ontology/LOAN/LoansSpecific/CardAccounts/> ;
	skos:definition "account holder to whom a payment card is issued" ;
	cmns-av:adaptedFrom "https://www.pcisecuritystandards.org/pci_security/glossary"^^xsd:anyURI ;
	.

fibo-loan-spc-crd:CreditCard
	a owl:Class ;
	rdfs:subClassOf
		fibo-loan-spc-crd:PaymentCard ,
		[
			a owl:Restriction ;
			owl:onProperty fibo-fnd-agr-ctr:isEvidenceFor ;
			owl:onClass fibo-loan-spc-crd:CreditCardAccount ;
			owl:qualifiedCardinality "1"^^xsd:nonNegativeInteger ;
		] ,
		[
			a owl:Restriction ;
			owl:onProperty cmns-cls:isClassifiedBy ;
			owl:someValuesFrom fibo-loan-spc-crd:CreditCardProduct ;
		]
		;
	rdfs:label "credit card" ;
	rdfs:isDefinedBy <https://spec.edmcouncil.org/fibo/ontology/LOAN/LoansSpecific/CardAccounts/> ;
	skos:definition "card issued by a financial service provider that enables the cardholder to borrow funds" ;
	cmns-av:explanatoryNote "Issuance of credit cards has the condition that the cardholder will pay back the original, borrowed amount plus any additional agreed-upon charges. The credit company provider may also grant a line of credit (LOC) to the cardholder which allows the holder to borrow money in the form of a cash advance. The issuer pre-sets borrowing limits which have a basis on the individual's credit rating." ;
	.

fibo-loan-spc-crd:CreditCardAccount
	a owl:Class ;
	rdfs:subClassOf
		fibo-fbc-pas-caa:LoanOrCreditAccount ,
		fibo-loan-spc-crd:CardAccount ,
		[
			a owl:Restriction ;
			owl:onProperty fibo-fbc-pas-caa:hasPaymentDueDate ;
			owl:someValuesFrom fibo-fbc-pas-caa:PaymentDueDate ;
		] ,
		[
			a owl:Restriction ;
			owl:onProperty fibo-fbc-pas-caa:realizes ;
			owl:someValuesFrom fibo-loan-spc-crd:CreditCardProduct ;
		] ,
		[
			a owl:Restriction ;
			owl:onProperty cmns-dsg:isDefinedIn ;
			owl:someValuesFrom fibo-loan-spc-crd:CreditCardAgreement ;
		] ,
		[
			a owl:Restriction ;
			owl:onProperty cmns-dsg:isSignifiedBy ;
			owl:someValuesFrom fibo-loan-spc-crd:CreditCard ;
		]
		;
	rdfs:label "credit card account" ;
	rdfs:isDefinedBy <https://spec.edmcouncil.org/fibo/ontology/LOAN/LoansSpecific/CardAccounts/> ;
	skos:definition "card account whose terms and conditions are defined in a credit card agreement that is represented by a credit card" ;
	.

fibo-loan-spc-crd:CreditCardAgreement
	a owl:Class ;
	rdfs:subClassOf
		fibo-fbc-dae-dbt:CommittedCreditFacility ,
		fibo-loan-spc-crd:PaymentCardAgreement ,
		[
			a owl:Restriction ;
			owl:onProperty fibo-fbc-dae-dbt:hasBorrower ;
			owl:someValuesFrom fibo-loan-spc-crd:Cardholder ;
		] ,
		[
			a owl:Restriction ;
			owl:onProperty fibo-fbc-dae-dbt:hasLender ;
			owl:someValuesFrom fibo-loan-spc-crd:IssuingFinancialInstitution ;
		] ,
		[
			a owl:Restriction ;
			owl:onProperty fibo-fnd-agr-ctr:isEvidencedBy ;
			owl:someValuesFrom fibo-loan-spc-crd:CreditCard ;
		] ,
		[
			a owl:Restriction ;
			owl:onProperty cmns-cxtdsg:appliesTo ;
			owl:someValuesFrom fibo-loan-spc-crd:CreditCardAccount ;
		]
		;
	rdfs:label "credit card agreement" ;
	rdfs:isDefinedBy <https://spec.edmcouncil.org/fibo/ontology/LOAN/LoansSpecific/CardAccounts/> ;
	skos:definition "account-specific credit facility that specifies the terms and conditions under which the credit card is offered to the cardholder by the issuer" ;
	.

fibo-loan-spc-crd:CreditCardNetwork
	a owl:Class ;
	rdfs:subClassOf
		cmns-cls:Classifier ,
		[
			a owl:Restriction ;
			owl:onProperty fibo-fnd-rel-rel:hasTag ;
			owl:someValuesFrom xsd:string ;
		] ,
		[
			a owl:Restriction ;
			owl:onProperty cmns-cls:classifies ;
			owl:someValuesFrom fibo-loan-spc-crd:CardProduct ;
		]
		;
	rdfs:label "credit card network" ;
	rdfs:isDefinedBy <https://spec.edmcouncil.org/fibo/ontology/LOAN/LoansSpecific/CardAccounts/> ;
	skos:definition "classifier for the network that authorizes, processes, and sets the terms of credit card transactions, as well as transfers payments between shoppers, merchants, and their banks" ;
	skos:example "Mastercard, Visa, American Express, Discover" ;
	.

fibo-loan-spc-crd:CreditCardProduct
	a owl:Class ;
	rdfs:subClassOf
		fibo-loan-spc-crd:CardProduct ,
		[
			a owl:Restriction ;
			owl:onProperty fibo-loan-spc-crd:hasCreditCardNetwork ;
			owl:onClass fibo-loan-spc-crd:CreditCardNetwork ;
			owl:qualifiedCardinality "1"^^xsd:nonNegativeInteger ;
		] ,
		[
			a owl:Restriction ;
			owl:onProperty fibo-fbc-pas-caa:isRealizedBy ;
			owl:someValuesFrom fibo-loan-spc-crd:CreditCardAccount ;
		] ,
		[
			a owl:Restriction ;
			owl:onProperty cmns-cls:classifies ;
			owl:someValuesFrom fibo-loan-spc-crd:CreditCard ;
		]
		;
	rdfs:label "credit card product" ;
	rdfs:isDefinedBy <https://spec.edmcouncil.org/fibo/ontology/LOAN/LoansSpecific/CardAccounts/> ;
	skos:definition "card product allowing the holder to purchase goods or services on credit" ;
	.

fibo-loan-spc-crd:DebitCard
	a owl:Class ;
	rdfs:subClassOf
		fibo-loan-spc-crd:PaymentCard ,
		[
			a owl:Restriction ;
			owl:onProperty fibo-fnd-agr-ctr:isEvidenceFor ;
			owl:onClass fibo-loan-spc-crd:DebitCardAccount ;
			owl:qualifiedCardinality "1"^^xsd:nonNegativeInteger ;
		] ,
		[
			a owl:Restriction ;
			owl:onProperty cmns-cls:isClassifiedBy ;
			owl:someValuesFrom fibo-loan-spc-crd:DebitCardProduct ;
		]
		;
	rdfs:label "debit card" ;
	rdfs:isDefinedBy <https://spec.edmcouncil.org/fibo/ontology/LOAN/LoansSpecific/CardAccounts/> ;
	skos:definition "payment card issued by a financial service provider that enables the cardholder to access funds in a demand deposit account" ;
	.

fibo-loan-spc-crd:DebitCardAccount
	a owl:Class ;
	rdfs:subClassOf
		fibo-loan-spc-crd:CardAccount ,
		[
			a owl:Restriction ;
			owl:onProperty fibo-fbc-pas-caa:realizes ;
			owl:someValuesFrom fibo-loan-spc-crd:DebitCardProduct ;
		] ,
		[
			a owl:Restriction ;
			owl:onProperty cmns-dsg:isSignifiedBy ;
			owl:someValuesFrom fibo-loan-spc-crd:DebitCard ;
		]
		;
	rdfs:label "debit card account" ;
	rdfs:isDefinedBy <https://spec.edmcouncil.org/fibo/ontology/LOAN/LoansSpecific/CardAccounts/> ;
	skos:definition "card account that is represented by a one or more debit cards" ;
	.

fibo-loan-spc-crd:DebitCardProduct
	a owl:Class ;
	rdfs:subClassOf
		fibo-loan-spc-crd:CardProduct ,
		[
			a owl:Restriction ;
			owl:onProperty fibo-fbc-pas-caa:isRealizedBy ;
			owl:someValuesFrom fibo-loan-spc-crd:DebitCardAccount ;
		] ,
		[
			a owl:Restriction ;
			owl:onProperty cmns-cls:classifies ;
			owl:someValuesFrom fibo-loan-spc-crd:DebitCard ;
		]
		;
	rdfs:label "debit card product" ;
	rdfs:isDefinedBy <https://spec.edmcouncil.org/fibo/ontology/LOAN/LoansSpecific/CardAccounts/> ;
	skos:definition "card product card typically provided by a depository institution allowing the holder to transfer money electronically to another account when making a purchase" ;
	.

fibo-loan-spc-crd:DiscoverNetwork
	a
		owl:NamedIndividual ,
		fibo-loan-spc-crd:CreditCardNetwork
		;
	rdfs:label "Discover network" ;
	rdfs:isDefinedBy <https://spec.edmcouncil.org/fibo/ontology/LOAN/LoansSpecific/CardAccounts/> ;
	skos:definition "credit card network and card issuer offering benefits like secondary rental car collision insurance" ;
	.

fibo-loan-spc-crd:IssuingFinancialInstitution
	a owl:Class ;
	rdfs:subClassOf
		fibo-fbc-fi-fi:Issuer ,
		fibo-fbc-pas-fpas:FinancialServiceProvider
		;
	rdfs:label "issuing financial institution" ;
	rdfs:isDefinedBy <https://spec.edmcouncil.org/fibo/ontology/LOAN/LoansSpecific/CardAccounts/> ;
	skos:definition "issuer and financial services provider that issues payment cards or performs, facilitates, or supports issuing services including but not limited to issuing banks and issuing processors" ;
	cmns-av:adaptedFrom "https://www.pcisecuritystandards.org/pci_security/glossary"^^xsd:anyURI ;
	cmns-av:synonym "issuing bank" ;
	.

fibo-loan-spc-crd:JCBNetwork
	a
		owl:NamedIndividual ,
		fibo-loan-spc-crd:CreditCardNetwork
		;
	rdfs:label "JCB network" ;
	rdfs:isDefinedBy <https://spec.edmcouncil.org/fibo/ontology/LOAN/LoansSpecific/CardAccounts/> ;
	skos:definition "credit card network based in Japan, with coverage throughout Asia, with strategic partners worldwide" ;
	cmns-av:explanatoryNote "JCB Co., Ltd., (formerly Japan Credit Bureau) is a credit card company based in Tokyo, Japan. As of 2020, it operates in 23 countries with over 130 million customers. In the United States, it is not a primary credit card network but has an association with the Discover Network to enable use of JCB cards." ;
	.

fibo-loan-spc-crd:MagneticStripeVerificationCodeValue
	a owl:Class ;
	rdfs:subClassOf fibo-loan-spc-crd:CardVerificationCodeValue ;
	rdfs:label "magnetic stripe verification code or value" ;
	rdfs:isDefinedBy <https://spec.edmcouncil.org/fibo/ontology/LOAN/LoansSpecific/CardAccounts/> ;
	skos:definition "card verification code on a card's magnetic stripe that uses secure cryptographic processes to protect data integrity on the stripe, and reveals any alteration or counterfeiting" ;
	cmns-av:adaptedFrom "https://www.pcisecuritystandards.org/pci_security/glossary"^^xsd:anyURI ;
	.

fibo-loan-spc-crd:MastercardNetwork
	a
		owl:NamedIndividual ,
		fibo-loan-spc-crd:CreditCardNetwork
		;
	rdfs:label "Mastercard network" ;
	rdfs:isDefinedBy <https://spec.edmcouncil.org/fibo/ontology/LOAN/LoansSpecific/CardAccounts/> ;
	skos:definition "credit card network that has its own suite of card protections and benefits, such as identity theft protection and extended warranties" ;
	.

fibo-loan-spc-crd:PaymentCard
	a owl:Class ;
	rdfs:subClassOf
		fibo-fnd-arr-doc:LegalDocument ,
		[
			a owl:Restriction ;
			owl:onProperty fibo-fnd-arr-doc:hasExpirationDate ;
			owl:onClass fibo-loan-spc-crd:CardExpirationDate ;
			owl:qualifiedCardinality "1"^^xsd:nonNegativeInteger ;
		] ,
		[
			a owl:Restriction ;
			owl:onProperty fibo-loan-spc-crd:hasCardVerificationCode ;
			owl:onClass fibo-loan-spc-crd:CardVerificationCodeValue ;
			owl:qualifiedCardinality "1"^^xsd:nonNegativeInteger ;
		] ,
		[
			a owl:Restriction ;
			owl:onProperty fibo-loan-spc-crd:hasPrimaryAccountNumber ;
			owl:onClass fibo-loan-spc-crd:PrimaryCardAccountNumber ;
			owl:qualifiedCardinality "1"^^xsd:nonNegativeInteger ;
		] ,
		[
			a owl:Restriction ;
			owl:onProperty fibo-fnd-agr-ctr:isEvidenceFor ;
			owl:someValuesFrom fibo-loan-spc-crd:CardAccount ;
		]
		;
	rdfs:label "payment card" ;
	rdfs:isDefinedBy <https://spec.edmcouncil.org/fibo/ontology/LOAN/LoansSpecific/CardAccounts/> ;
	rdfs:seeAlso <https://www.irs.gov/payments/payment-card-transactions-faqs> ;
	skos:definition "legal document issued by a financial services provider that enables the cardholder to access the funds in the customer's designated bank accounts, or through a credit account and make payments by electronic funds transfer and access automated teller machines (ATMs)" ;
	cmns-av:explanatoryNote
		"For purposes of Payment Card Industry Data Security Standard (PCI DSS), a payment card is any payment card/device that bears the logo of the founding members of PCI SSC, which are American Express, Discover Financial Services, JCB International, MasterCard, or Visa, Inc." ,
		"The term payment card includes credit cards, debit cards, and stored-value cards, as well as payment through any distinctive marks of a payment card (such as a credit card number). A payment card is issued under an agreement that provides standards and mechanisms for settling the transactions between a merchant acquiring bank or similar entity and the providers who accept the cards as payment."
		;
	.

fibo-loan-spc-crd:PaymentCardAgreement
	a owl:Class ;
	rdfs:subClassOf
		fibo-fbc-dae-dbt:CreditAgreement ,
		fibo-fbc-pas-caa:AccountSpecificServiceAgreement ,
		[
			a owl:Restriction ;
			owl:onProperty fibo-fnd-agr-ctr:hasContractParty ;
			owl:someValuesFrom fibo-loan-spc-crd:Cardholder ;
		] ,
		[
			a owl:Restriction ;
			owl:onProperty fibo-fnd-agr-ctr:hasContractParty ;
			owl:someValuesFrom fibo-loan-spc-crd:IssuingFinancialInstitution ;
		] ,
		[
			a owl:Restriction ;
			owl:onProperty fibo-fnd-agr-ctr:isEvidencedBy ;
			owl:someValuesFrom fibo-loan-spc-crd:PaymentCard ;
		] ,
		[
			a owl:Restriction ;
			owl:onProperty cmns-cxtdsg:appliesTo ;
			owl:someValuesFrom fibo-loan-spc-crd:CardAccount ;
		]
		;
	rdfs:label "payment card agreement" ;
	rdfs:isDefinedBy <https://spec.edmcouncil.org/fibo/ontology/LOAN/LoansSpecific/CardAccounts/> ;
	skos:definition "account-specific credit agreement that specifies the terms and conditions under which the payment card is offered to the cardholder by the issuer" ;
	.

fibo-loan-spc-crd:PrimaryCardAccountNumber
	a owl:Class ;
	rdfs:subClassOf
		fibo-fbc-pas-caa:AccountIdentifier ,
		[
			a owl:Restriction ;
			owl:onProperty cmns-id:identifies ;
			owl:onClass fibo-loan-spc-crd:CardAccount ;
			owl:qualifiedCardinality "1"^^xsd:nonNegativeInteger ;
		]
		;
	rdfs:label "primary card account number" ;
	rdfs:isDefinedBy <https://spec.edmcouncil.org/fibo/ontology/LOAN/LoansSpecific/CardAccounts/> ;
	skos:definition "composite identifier of 14 or 16 digits embossed on a bank or payment card and encoded in the card's magnetic strip" ;
	cmns-av:abbreviation "PAN" ;
	cmns-av:explanatoryNote "The PAN identifies the issuer of the card and the account including part of the account number, and contains a check digit that verifies the authenticity of the embossed account number." ;
	cmns-av:synonym "primary account number" ;
	.

fibo-loan-spc-crd:SmartCard
	a owl:Class ;
	rdfs:subClassOf fibo-loan-spc-crd:PaymentCard ;
	rdfs:label "smart card" ;
	rdfs:isDefinedBy <https://spec.edmcouncil.org/fibo/ontology/LOAN/LoansSpecific/CardAccounts/> ;
	skos:definition "payment card that has integrated circuits embedded within it" ;
	cmns-av:adaptedFrom "https://www.pcisecuritystandards.org/pci_security/glossary"^^xsd:anyURI ;
	cmns-av:explanatoryNote "The circuits, also referred to as the 'chip,' contain payment card data including but not limited to data equivalent to the magnetic-stripe data." ;
	.

fibo-loan-spc-crd:ThreeDigitVerificationCodeValue
	a owl:Class ;
	rdfs:subClassOf fibo-loan-spc-crd:CardVerificationCodeValue ;
	rdfs:label "three-digit verification code or value" ;
	rdfs:isDefinedBy <https://spec.edmcouncil.org/fibo/ontology/LOAN/LoansSpecific/CardAccounts/> ;
	skos:definition "card verification code that is the rightmost three-digit value printed in the signature panel area on the back of the card" ;
	cmns-av:adaptedFrom "https://www.pcisecuritystandards.org/pci_security/glossary"^^xsd:anyURI ;
	.

fibo-loan-spc-crd:VisaNetwork
	a
		owl:NamedIndividual ,
		fibo-loan-spc-crd:CreditCardNetwork
		;
	rdfs:label "Visa network" ;
	rdfs:isDefinedBy <https://spec.edmcouncil.org/fibo/ontology/LOAN/LoansSpecific/CardAccounts/> ;
	skos:definition "credit card network that oversees the Visa Signature benefits associated with certain credit cards, such as premium rental car privileges and hotel perks" ;
	.

fibo-loan-spc-crd:hasCardVerificationCode
	a owl:ObjectProperty ;
	rdfs:label "has card verification code" ;
	rdfs:domain fibo-loan-spc-crd:PaymentCard ;
	rdfs:isDefinedBy <https://spec.edmcouncil.org/fibo/ontology/LOAN/LoansSpecific/CardAccounts/> ;
	rdfs:range fibo-loan-spc-crd:CardVerificationCodeValue ;
	skos:definition "links a credit card to either: (1) magnetic-stripe data, or (2) printed security features that are used to protect data integrity and limit alteration, counterfeiting and fraud generally" ;
	.

fibo-loan-spc-crd:hasCreditCardNetwork
	a owl:ObjectProperty ;
	rdfs:subPropertyOf cmns-cls:isClassifiedBy ;
	rdfs:label "has credit card network" ;
	rdfs:isDefinedBy <https://spec.edmcouncil.org/fibo/ontology/LOAN/LoansSpecific/CardAccounts/> ;
	rdfs:range fibo-loan-spc-crd:CreditCardNetwork ;
	skos:definition "indicates the underlying network for credit card product" ;
	.

fibo-loan-spc-crd:hasPrimaryAccountNumber
	a owl:ObjectProperty ;
	rdfs:label "has primary account number" ;
	rdfs:domain fibo-loan-spc-crd:PaymentCard ;
	rdfs:isDefinedBy <https://spec.edmcouncil.org/fibo/ontology/LOAN/LoansSpecific/CardAccounts/> ;
	rdfs:range fibo-loan-spc-crd:PrimaryCardAccountNumber ;
	skos:definition "specifies the account number displayed on the face of the card" ;
	skos:editorialNote "modeled independently of 'identifies' in order to circumvent circular reasoning challenges" ;
	.

fibo-loan-spc-crd:usesCurrency
	a owl:ObjectProperty ;
	rdfs:subPropertyOf cmns-cxtdsg:uses ;
	rdfs:label "uses currency" ;
	rdfs:isDefinedBy <https://spec.edmcouncil.org/fibo/ontology/LOAN/LoansSpecific/CardAccounts/> ;
	rdfs:range fibo-fnd-acc-cur:Currency ;
	skos:definition "indicates the currency defined for the credit card product" ;
	.

