# baseURI: https://spec.edmcouncil.org/fibo/ontology/master/2023Q2/FND/Parties/Parties/
# imports: https://spec.edmcouncil.org/fibo/ontology/master/2023Q2/FND/AgentsAndPeople/Agents/
# imports: https://spec.edmcouncil.org/fibo/ontology/master/2023Q2/FND/DatesAndTimes/BusinessDates/
# imports: https://spec.edmcouncil.org/fibo/ontology/master/2023Q2/FND/Parties/Roles/
# imports: https://spec.edmcouncil.org/fibo/ontology/master/2023Q2/FND/Places/Addresses/
# imports: https://spec.edmcouncil.org/fibo/ontology/master/2023Q2/FND/Relations/Relations/
# imports: https://spec.edmcouncil.org/fibo/ontology/master/2023Q2/FND/Utilities/AnnotationVocabulary/
# imports: https://www.omg.org/spec/Commons/AnnotationVocabulary/
# imports: https://www.omg.org/spec/Commons/Collections/
# imports: https://www.omg.org/spec/Commons/ContextualDesignators/
# imports: https://www.omg.org/spec/Commons/DatesAndTimes/
# imports: https://www.omg.org/spec/Commons/Designators/
# imports: https://www.omg.org/spec/Commons/Identifiers/

@base <https://spec.edmcouncil.org/fibo/ontology/master/2023Q2/FND/Parties/Parties/> .
@prefix cmns-av: <https://www.omg.org/spec/Commons/AnnotationVocabulary/> .
@prefix cmns-col: <https://www.omg.org/spec/Commons/Collections/> .
@prefix cmns-cxtdsg: <https://www.omg.org/spec/Commons/ContextualDesignators/> .
@prefix cmns-dsg: <https://www.omg.org/spec/Commons/Designators/> .
@prefix cmns-dt: <https://www.omg.org/spec/Commons/DatesAndTimes/> .
@prefix cmns-id: <https://www.omg.org/spec/Commons/Identifiers/> .
@prefix dcterms: <http://purl.org/dc/terms/> .
@prefix fibo-fnd-aap-agt: <https://spec.edmcouncil.org/fibo/ontology/FND/AgentsAndPeople/Agents/> .
@prefix fibo-fnd-dt-bd: <https://spec.edmcouncil.org/fibo/ontology/FND/DatesAndTimes/BusinessDates/> .
@prefix fibo-fnd-plc-adr: <https://spec.edmcouncil.org/fibo/ontology/FND/Places/Addresses/> .
@prefix fibo-fnd-pty-pty: <https://spec.edmcouncil.org/fibo/ontology/FND/Parties/Parties/> .
@prefix fibo-fnd-pty-rl: <https://spec.edmcouncil.org/fibo/ontology/FND/Parties/Roles/> .
@prefix fibo-fnd-rel-rel: <https://spec.edmcouncil.org/fibo/ontology/FND/Relations/Relations/> .
@prefix fibo-fnd-utl-av: <https://spec.edmcouncil.org/fibo/ontology/FND/Utilities/AnnotationVocabulary/> .
@prefix owl: <http://www.w3.org/2002/07/owl#> .
@prefix rdf: <http://www.w3.org/1999/02/22-rdf-syntax-ns#> .
@prefix rdfs: <http://www.w3.org/2000/01/rdf-schema#> .
@prefix skos: <http://www.w3.org/2004/02/skos/core#> .
@prefix xsd: <http://www.w3.org/2001/XMLSchema#> .

<https://spec.edmcouncil.org/fibo/ontology/FND/Parties/Parties/>
	a owl:Ontology ;
	rdfs:label "Parties Ontology" ;
	dcterms:abstract "This ontology defines the high-level concepts for party roles. The concept of a party in a role describes some entity defined specifically in terms of one or more roles it performs in situations and other relationships such as some formal contractual or transactional relationship." ;
	dcterms:license "https://opensource.org/licenses/MIT"^^xsd:anyURI ;
	owl:imports
		<https://spec.edmcouncil.org/fibo/ontology/master/2023Q2/FND/AgentsAndPeople/Agents/> ,
		<https://spec.edmcouncil.org/fibo/ontology/master/2023Q2/FND/DatesAndTimes/BusinessDates/> ,
		<https://spec.edmcouncil.org/fibo/ontology/master/2023Q2/FND/Parties/Roles/> ,
		<https://spec.edmcouncil.org/fibo/ontology/master/2023Q2/FND/Places/Addresses/> ,
		<https://spec.edmcouncil.org/fibo/ontology/master/2023Q2/FND/Relations/Relations/> ,
		<https://spec.edmcouncil.org/fibo/ontology/master/2023Q2/FND/Utilities/AnnotationVocabulary/> ,
		<https://www.omg.org/spec/Commons/AnnotationVocabulary/> ,
		<https://www.omg.org/spec/Commons/Collections/> ,
		<https://www.omg.org/spec/Commons/ContextualDesignators/> ,
		<https://www.omg.org/spec/Commons/DatesAndTimes/> ,
		<https://www.omg.org/spec/Commons/Designators/> ,
		<https://www.omg.org/spec/Commons/Identifiers/>
		;
	owl:versionIRI <https://spec.edmcouncil.org/fibo/ontology/master/2023Q2/FND/Parties/Parties/> ;
	skos:changeNote
		"The http://www.omg.org/spec/EDMC-FIBO/FND/20130801/Parties/Parties.rdf version of the ontology was was modified per the issue resolutions identified in the FIBO FND 1.0 FTF report and in https://spec.edmcouncil.org/fibo/ontology/FND/1.0/AboutFND-1.0/." ,
		"The http://www.omg.org/spec/EDMC-FIBO/FND/20141101/Parties/Parties.rdf version of this ontology was revised as a part of the issue resolutions identified in the FIBO FND 1.1 RTF report to add a parent of hasDate to date properties." ,
		"The http://www.omg.org/spec/EDMC-FIBO/FND/20160201/Parties/Parties.rdf version of this ontology was revised as a part of the FIBO 2.0 RFC to introduce disjointness axioms to aid users in understanding." ,
		"""The http://www.omg.org/spec/FIBO/Foundations/20130601/Roles/Parties.owl version of the ontology was revised in advance of the September 2013 New Brunswick, NJ meeting, as follows:
	(1) to use slash style URI/IRIss (also called 303 URIs, vs. hash style) as required to support server side processing 
	(2) to use version-independent IRIs for all definitions internally as opposed to version-specific IRIs
	(3) to change the file suffix from .owl to .rdf to increase usability in RDF tools
	(4) to use 4-level abbreviations and corresponding namespace prefixes for all FIBO ontologies, reflecting a family/specification/module/ontology structure
	(5) to incorporate changes to the specification metadata to support documentation at the family, specification, module, and ontology level, similar to the abbreviations.
	(6) to combine Parties, Party Roles, and Roles in a single, new, Parties module, combine Parties and Party Roles into a single ontology, and add an inverse for the hasParty property.""" ,
		"The https://spec.edmcouncil.org/fibo/ontology/FND/Parties/Parties.rdf version of the ontology was modified to use the Commons Ontology Library (Commons) Annotation Vocabulary rather than the OMG's Specification Metadata vocabulary." ,
		"The https://spec.edmcouncil.org/fibo/ontology/FND/Parties/Parties.rdf version of this ontology was extended to add the concepts of tax identifier and tax identification scheme." ,
		"The https://spec.edmcouncil.org/fibo/ontology/FND/Parties/Parties.rdf version of this ontology was extended to align the properties holds and isHeldBy with the lattice to improve ownership-related reasoning." ,
		"The https://spec.edmcouncil.org/fibo/ontology/FND/Parties/Parties.rdf version of this ontology was extended to rename 'hasPrimaryParty' to 'hasActiveParty' to be more consistent." ,
		"The https://spec.edmcouncil.org/fibo/ontology/FND/Parties/Parties.rdf version of this ontology was extended to support more complex situations involving parties in various roles, loosen the restriction on party in role with respect to commencement date, and to eliminate the redundant union in the definition of independent party." ,
		"The https://spec.edmcouncil.org/fibo/ontology/FND/Parties/Parties.rdf version of this ontology was modified to use the Commons Ontology Library (Commons) rather than the OMG's Languages, Countries and Codes (LCC) and to eliminate redundancies in FIBO as appropriate." ,
		"The https://spec.edmcouncil.org/fibo/ontology/FND/Parties/Parties.rdf version of this ontology was revised to add a relationship directly between parties and a party identifier and rename (migrate) the hasDefinition property to isDefinedIn to clarify intent." ,
		"The https://spec.edmcouncil.org/fibo/ontology/FND/Parties/Parties.rdf version of this ontology was revised to add semantics to the definition of independent party, making it a direct subclass of autonomous agent (rather than inferred only) and making person and organization direct subclasses (rather than inferred only)." ,
		"The https://spec.edmcouncil.org/fibo/ontology/FND/Parties/Parties.rdf version of this ontology was revised to add the two remaining property chains to complete the lattice, from independent party to thing via the situation, to simplify the class hierarchy for improved understanding, data mapping and alignment, and to add the notion of a contextual name (i.e., a name for someone, some place or something that applies for some period of time in some context)." ,
		"The https://spec.edmcouncil.org/fibo/ontology/FND/Parties/Parties.rdf version of this ontology was revised to address hygiene issues with respect to text formatting." ,
		"The https://spec.edmcouncil.org/fibo/ontology/FND/Parties/Parties.rdf version of this ontology was revised to eliminate duplication with the concepts in LCC." ,
		"The https://spec.edmcouncil.org/fibo/ontology/FND/Parties/Parties.rdf version of this ontology was revised to make hasRelatedPartyInRole symmetric and move hasMailingAddress from people to this ontology."
		;
	fibo-fnd-utl-av:hasMaturityLevel fibo-fnd-utl-av:Release ;
	cmns-av:copyright
		"Copyright (c) 2013-2023 EDM Council, Inc." ,
		"Copyright (c) 2013-2023 Object Management Group, Inc."
		;
	.

fibo-fnd-pty-pty:Actor
	a owl:Class ;
	rdfs:subClassOf fibo-fnd-pty-pty:PartyInRole ;
	rdfs:label "actor" ;
	rdfs:isDefinedBy <https://spec.edmcouncil.org/fibo/ontology/FND/Parties/Parties/> ;
	skos:definition "party that is the primary performer in a relationship between parties, i.e., the party that does something, causes something to happen, or otherwise plays an agentive role in the relationship" ;
	skos:example "Examples include owner, controlling party, beneficiary, guarantor, partner in a partnership, shareholder, etc." ;
	.

fibo-fnd-pty-pty:ContextualName
	a owl:Class ;
	rdfs:isDefinedBy <https://spec.edmcouncil.org/fibo/ontology/FND/Parties/Parties/> ;
	owl:deprecated "true"^^xsd:boolean ;
	owl:equivalentClass cmns-cxtdsg:ContextualName ;
	.

fibo-fnd-pty-pty:IndependentParty
	a owl:Class ;
	rdfs:subClassOf
		fibo-fnd-aap-agt:AutonomousAgent ,
		[
			a owl:Restriction ;
			owl:onProperty fibo-fnd-pty-pty:hasMailingAddress ;
			owl:onClass fibo-fnd-plc-adr:PhysicalAddress ;
			owl:minQualifiedCardinality "0"^^xsd:nonNegativeInteger ;
		] ,
		[
			a owl:Restriction ;
			owl:onProperty fibo-fnd-plc-adr:hasAddress ;
			owl:onClass fibo-fnd-plc-adr:PhysicalAddress ;
			owl:minQualifiedCardinality "0"^^xsd:nonNegativeInteger ;
		]
		;
	rdfs:label "independent party" ;
	rdfs:isDefinedBy <https://spec.edmcouncil.org/fibo/ontology/FND/Parties/Parties/> ;
	owl:disjointWith fibo-fnd-pty-rl:AgentInRole ;
	skos:definition "any person or organization" ;
	.

fibo-fnd-pty-pty:PartyInRole
	a owl:Class ;
	rdfs:subClassOf
		fibo-fnd-pty-rl:AgentInRole ,
		[
			a owl:Restriction ;
			owl:onProperty fibo-fnd-pty-pty:hasCommencementDate ;
			owl:onClass cmns-dt:Date ;
			owl:minQualifiedCardinality "0"^^xsd:nonNegativeInteger ;
		] ,
		[
			a owl:Restriction ;
			owl:onProperty fibo-fnd-rel-rel:hasIdentity ;
			owl:onClass fibo-fnd-pty-pty:IndependentParty ;
			owl:qualifiedCardinality "1"^^xsd:nonNegativeInteger ;
		]
		;
	rdfs:label "party in role" ;
	rdfs:isDefinedBy <https://spec.edmcouncil.org/fibo/ontology/FND/Parties/Parties/> ;
	skos:definition "relative concept that ties a person or organization to a specific role they stand in" ;
	skos:example "Examples include organization member, issuer, owner, partner in a partnership, shareholder, etc." ;
	skos:scopeNote "The concept of a party in a role refers only to those contexts in which in natural English one would call someone a 'party' for example being party to a contract or to a transaction; it does not cover entities as performing some role in some activity or process (the separate concept Actor covers that). A good test is whether the relative thing defined as PartyInRole can be sensibly said to have a part or play a part in something. Corresponds to the English (not data modeling) sense of the word 'Party'." ;
	cmns-av:adaptedFrom "OMG Property and Casualty Information Models, dtc/12-01-04, Annex A, Glossary of Data Model Terms and Definitions" ;
	.

fibo-fnd-pty-pty:PartyInRoleIdentificationScheme
	a owl:Class ;
	rdfs:subClassOf
		cmns-id:IdentificationScheme ,
		[
			a owl:Restriction ;
			owl:onProperty cmns-col:hasMember ;
			owl:someValuesFrom fibo-fnd-pty-pty:PartyInRoleIdentifier ;
		]
		;
	rdfs:label "party-in-role identification scheme" ;
	rdfs:isDefinedBy <https://spec.edmcouncil.org/fibo/ontology/FND/Parties/Parties/> ;
	skos:definition "system for allocating identifiers to parties" ;
	.

fibo-fnd-pty-pty:PartyInRoleIdentifier
	a owl:Class ;
	rdfs:subClassOf
		cmns-id:Identifier ,
		[
			a owl:Restriction ;
			owl:onProperty cmns-id:identifies ;
			owl:onClass fibo-fnd-pty-pty:PartyInRole ;
			owl:qualifiedCardinality "1"^^xsd:nonNegativeInteger ;
		] ,
		[
			a owl:Restriction ;
			owl:onProperty cmns-col:isMemberOf ;
			owl:onClass fibo-fnd-pty-pty:PartyInRoleIdentificationScheme ;
			owl:qualifiedCardinality "1"^^xsd:nonNegativeInteger ;
		] ,
		[
			a owl:Restriction ;
			owl:onProperty cmns-dsg:isDefinedIn ;
			owl:onClass fibo-fnd-pty-pty:PartyInRoleIdentificationScheme ;
			owl:qualifiedCardinality "1"^^xsd:nonNegativeInteger ;
		]
		;
	rdfs:label "party-in-role identifier" ;
	rdfs:isDefinedBy <https://spec.edmcouncil.org/fibo/ontology/FND/Parties/Parties/> ;
	skos:definition "sequence of characters, capable of uniquely identifying a party based on a specific role that they play in some context" ;
	.

fibo-fnd-pty-pty:Situation
	a owl:Class ;
	rdfs:subClassOf
		[
			a owl:Restriction ;
			owl:onProperty fibo-fnd-pty-pty:hasUndergoer ;
			owl:onClass fibo-fnd-pty-pty:Undergoer ;
			owl:minQualifiedCardinality "0"^^xsd:nonNegativeInteger ;
		] ,
		[
			a owl:Restriction ;
			owl:onProperty fibo-fnd-dt-bd:holdsDuring ;
			owl:onClass cmns-dt:DatePeriod ;
			owl:minQualifiedCardinality "0"^^xsd:nonNegativeInteger ;
		] ,
		[
			a owl:Restriction ;
			owl:onProperty fibo-fnd-pty-pty:hasActor ;
			owl:someValuesFrom fibo-fnd-pty-pty:Actor ;
		]
		;
	rdfs:label "situation" ;
	rdfs:isDefinedBy <https://spec.edmcouncil.org/fibo/ontology/FND/Parties/Parties/> ;
	skos:definition "setting, state of being, or relationship that that is relatively stable for some period of time" ;
	skos:example "Examples include ownership, control, possession, affiliation, beneficiary, and other similar relations." ;
	cmns-av:usageNote "From a usage perspective, situations are essentially reified relations at the top of the FIBO relationship lattice, also known as mediating relationships." ;
	.

fibo-fnd-pty-pty:TaxIdentificationScheme
	a owl:Class ;
	rdfs:subClassOf cmns-id:IdentificationScheme ;
	rdfs:label "tax identification scheme" ;
	rdfs:isDefinedBy <https://spec.edmcouncil.org/fibo/ontology/FND/Parties/Parties/> ;
	skos:definition "identification scheme used to identify taxpayers in some jurisdiction" ;
	cmns-av:adaptedFrom "https://www.oecd-ilibrary.org/taxation/standard-for-automatic-exchange-of-financial-account-information-in-tax-matters-second-edition_9789264267992-en"^^xsd:anyURI ;
	.

fibo-fnd-pty-pty:TaxIdentifier
	a owl:Class ;
	rdfs:subClassOf
		cmns-id:Identifier ,
		[
			a owl:Restriction ;
			owl:onProperty cmns-id:identifies ;
			owl:onClass fibo-fnd-pty-pty:IndependentParty ;
			owl:qualifiedCardinality "1"^^xsd:nonNegativeInteger ;
		] ,
		[
			a owl:Restriction ;
			owl:onProperty cmns-col:isMemberOf ;
			owl:onClass fibo-fnd-pty-pty:TaxIdentificationScheme ;
			owl:qualifiedCardinality "1"^^xsd:nonNegativeInteger ;
		]
		;
	rdfs:label "tax identifier" ;
	rdfs:isDefinedBy <https://spec.edmcouncil.org/fibo/ontology/FND/Parties/Parties/> ;
	skos:definition "identifier assigned to a taxpayer that enables compulsory financial charges and other levies to be imposed on the taxpayer by a governmental organization in order to fund government spending and various public expenditures" ;
	cmns-av:adaptedFrom "https://www.oecd-ilibrary.org/taxation/standard-for-automatic-exchange-of-financial-account-information-in-tax-matters-second-edition_9789264267992-en"^^xsd:anyURI ;
	cmns-av:explanatoryNote "Tax identifiers are used for various tax-related purposes in the United States and in other countries under the Common Reporting Standard (CRS)." ;
	.

fibo-fnd-pty-pty:Undergoer
	a owl:Class ;
	rdfs:subClassOf fibo-fnd-pty-rl:ThingInRole ;
	rdfs:label "undergoer" ;
	rdfs:isDefinedBy <https://spec.edmcouncil.org/fibo/ontology/FND/Parties/Parties/> ;
	skos:definition "something that is the recipient in a relationship, i.e., the thing (or party) that something impacts, affects, or otherwise plays passive recipient / patient or theme role in the relationship" ;
	skos:example "Examples include something that is owned or controlled." ;
	.

fibo-fnd-pty-pty:actsIn
	a owl:ObjectProperty ;
	rdfs:label "acts in" ;
	rdfs:domain fibo-fnd-pty-pty:Actor ;
	rdfs:isDefinedBy <https://spec.edmcouncil.org/fibo/ontology/FND/Parties/Parties/> ;
	rdfs:range fibo-fnd-pty-pty:Situation ;
	owl:inverseOf fibo-fnd-pty-pty:hasActor ;
	skos:definition "indicates a situation in which the actor plays a primary role" ;
	.

fibo-fnd-pty-pty:actsOn
	a owl:ObjectProperty ;
	rdfs:label "acts on" ;
	rdfs:isDefinedBy <https://spec.edmcouncil.org/fibo/ontology/FND/Parties/Parties/> ;
	owl:propertyChainAxiom (
		fibo-fnd-pty-pty:actsIn
		fibo-fnd-pty-pty:hasUndergoer
	) ;
	skos:definition "relates an actor in a given situation to the undergoer that they affect under the circumstances" ;
	.

fibo-fnd-pty-pty:directlyAffects
	a owl:ObjectProperty ;
	rdfs:label "directly affects" ;
	rdfs:isDefinedBy <https://spec.edmcouncil.org/fibo/ontology/FND/Parties/Parties/> ;
	owl:inverseOf fibo-fnd-pty-pty:experiencesWith ;
	owl:propertyChainAxiom (
		fibo-fnd-pty-pty:actsIn
		fibo-fnd-pty-pty:hasUndergoer
		fibo-fnd-pty-rl:isPlayedBy
	) ;
	skos:definition "relates an actor in a given situation to the thing (or party) that they impact under the circumstances" ;
	.

fibo-fnd-pty-pty:experiences
	a owl:ObjectProperty ;
	rdfs:label "experiences" ;
	rdfs:isDefinedBy <https://spec.edmcouncil.org/fibo/ontology/FND/Parties/Parties/> ;
	owl:propertyChainAxiom (
		fibo-fnd-pty-rl:playsRole
		fibo-fnd-pty-pty:undergoes
	) ;
	skos:definition "relates something to a situation that affects them in some way" ;
	.

fibo-fnd-pty-pty:experiencesDirectly
	a owl:ObjectProperty ;
	rdfs:label "experiences directly" ;
	rdfs:isDefinedBy <https://spec.edmcouncil.org/fibo/ontology/FND/Parties/Parties/> ;
	owl:propertyChainAxiom (
		fibo-fnd-pty-rl:playsRole
		fibo-fnd-pty-pty:undergoes
		fibo-fnd-pty-pty:hasActor
		fibo-fnd-pty-rl:isPlayedBy
	) ;
	skos:definition "relates something directly to a party that drives a situation involving it" ;
	.

fibo-fnd-pty-pty:experiencesWith
	a owl:ObjectProperty ;
	rdfs:label "experiences with" ;
	rdfs:isDefinedBy <https://spec.edmcouncil.org/fibo/ontology/FND/Parties/Parties/> ;
	owl:propertyChainAxiom (
		fibo-fnd-pty-rl:playsRole
		fibo-fnd-pty-pty:undergoes
		fibo-fnd-pty-pty:hasActor
	) ;
	skos:definition "relates something to an actor that drives a situation involving it" ;
	.

fibo-fnd-pty-pty:hasActiveParty
	a owl:ObjectProperty ;
	rdfs:label "has active party" ;
	rdfs:isDefinedBy <https://spec.edmcouncil.org/fibo/ontology/FND/Parties/Parties/> ;
	owl:inverseOf fibo-fnd-pty-pty:playsActiveRoleIn ;
	owl:propertyChainAxiom (
		fibo-fnd-pty-pty:hasActor
		fibo-fnd-pty-rl:isPlayedBy
	) ;
	skos:definition "relates a situation to the person or organization acting in a primary (agentive) role" ;
	.

fibo-fnd-pty-pty:hasActor
	a owl:ObjectProperty ;
	rdfs:subPropertyOf fibo-fnd-pty-pty:hasPartyInRole ;
	rdfs:label "has actor" ;
	rdfs:domain fibo-fnd-pty-pty:Situation ;
	rdfs:isDefinedBy <https://spec.edmcouncil.org/fibo/ontology/FND/Parties/Parties/> ;
	rdfs:range fibo-fnd-pty-pty:Actor ;
	skos:definition "identifies the primary party acting in a specific role with respect to a given situation" ;
	.

fibo-fnd-pty-pty:hasCommencementDate
	a owl:ObjectProperty ;
	rdfs:subPropertyOf cmns-dt:hasStartDate ;
	rdfs:label "has commencement date" ;
	rdfs:domain fibo-fnd-pty-pty:PartyInRole ;
	rdfs:isDefinedBy <https://spec.edmcouncil.org/fibo/ontology/FND/Parties/Parties/> ;
	rdfs:range cmns-dt:Date ;
	skos:definition "the date a party relationship comes into force" ;
	.

fibo-fnd-pty-pty:hasMailingAddress
	a owl:ObjectProperty ;
	rdfs:subPropertyOf fibo-fnd-plc-adr:hasAddress ;
	rdfs:label "has mailing address" ;
	rdfs:domain fibo-fnd-pty-pty:IndependentParty ;
	rdfs:isDefinedBy <https://spec.edmcouncil.org/fibo/ontology/FND/Parties/Parties/> ;
	rdfs:range fibo-fnd-plc-adr:PhysicalAddress ;
	skos:definition "identifies a physical address where an independent party can receive communications, including letters and packages" ;
	.

fibo-fnd-pty-pty:hasParty
	a owl:ObjectProperty ;
	rdfs:label "has party" ;
	rdfs:isDefinedBy <https://spec.edmcouncil.org/fibo/ontology/FND/Parties/Parties/> ;
	rdfs:range fibo-fnd-pty-pty:IndependentParty ;
	skos:definition "identifies an independent party associated with an agreement, contract, policy, regulation, or other business arrangement" ;
	.

fibo-fnd-pty-pty:hasPartyInRole
	a owl:ObjectProperty ;
	rdfs:subPropertyOf fibo-fnd-pty-pty:hasThingInRole ;
	rdfs:label "has party in role" ;
	rdfs:isDefinedBy <https://spec.edmcouncil.org/fibo/ontology/FND/Parties/Parties/> ;
	rdfs:range fibo-fnd-pty-pty:PartyInRole ;
	skos:definition "identifies a party acting in a specific role as related to the particular agreement, contract, policy, regulation, or other business relationship" ;
	.

fibo-fnd-pty-pty:hasRelatedPartyInRole
	a
		owl:ObjectProperty ,
		owl:SymmetricProperty
		;
	rdfs:subPropertyOf fibo-fnd-pty-pty:hasPartyInRole ;
	rdfs:label "has related party-in-role" ;
	rdfs:domain fibo-fnd-pty-pty:PartyInRole ;
	rdfs:isDefinedBy <https://spec.edmcouncil.org/fibo/ontology/FND/Parties/Parties/> ;
	rdfs:range fibo-fnd-pty-pty:PartyInRole ;
	skos:definition "relates a party acting in a specific role directly to another party acting in the same or another role" ;
	cmns-av:usageNote "This property is intended as an abstract property, whose subproperties may or may not be symmetric, but could be inverses of one another." ;
	.

fibo-fnd-pty-pty:hasThingInRole
	a owl:ObjectProperty ;
	rdfs:label "has thing in role" ;
	rdfs:isDefinedBy <https://spec.edmcouncil.org/fibo/ontology/FND/Parties/Parties/> ;
	rdfs:range fibo-fnd-pty-rl:ThingInRole ;
	skos:definition "identifies something acting in a recipient or target role as related to the particular agreement, contract, policy, regulation, situation, or other business relationship" ;
	.

fibo-fnd-pty-pty:hasUndergoer
	a owl:ObjectProperty ;
	rdfs:subPropertyOf fibo-fnd-pty-pty:hasThingInRole ;
	rdfs:label "has undergoer" ;
	rdfs:domain fibo-fnd-pty-pty:Situation ;
	rdfs:isDefinedBy <https://spec.edmcouncil.org/fibo/ontology/FND/Parties/Parties/> ;
	rdfs:range fibo-fnd-pty-pty:Undergoer ;
	skos:definition "identifies the experiencer in a specific role with respect to a given situation" ;
	.

fibo-fnd-pty-pty:isAPartyTo
	a owl:ObjectProperty ;
	rdfs:label "is a party to" ;
	rdfs:domain fibo-fnd-pty-pty:IndependentParty ;
	rdfs:isDefinedBy <https://spec.edmcouncil.org/fibo/ontology/FND/Parties/Parties/> ;
	owl:inverseOf fibo-fnd-pty-pty:hasParty ;
	skos:definition "identifies an agreement, contract, policy, regulation, or other business transaction that an independent party is associated with" ;
	cmns-av:explanatoryNote "This property should be read referring to some context (known as a 'mediating thing' in the informative upper ontology)." ;
	.

fibo-fnd-pty-pty:isAffectedBy
	a owl:ObjectProperty ;
	rdfs:label "is affected by" ;
	rdfs:isDefinedBy <https://spec.edmcouncil.org/fibo/ontology/FND/Parties/Parties/> ;
	owl:propertyChainAxiom (
		fibo-fnd-pty-pty:undergoes
		fibo-fnd-pty-pty:hasActor
	) ;
	skos:definition "relates an undergoer in a given situation to the actor that has an impact on them under the circumstances" ;
	.

fibo-fnd-pty-pty:isDirectlyAffectedBy
	a owl:ObjectProperty ;
	rdfs:label "is directly affected by" ;
	rdfs:isDefinedBy <https://spec.edmcouncil.org/fibo/ontology/FND/Parties/Parties/> ;
	owl:propertyChainAxiom (
		fibo-fnd-pty-pty:undergoes
		fibo-fnd-pty-pty:hasActor
		fibo-fnd-pty-rl:isPlayedBy
	) ;
	skos:definition "relates an undergoer in a given situation to the person or organization that has an impact on them under the circumstances" ;
	.

fibo-fnd-pty-pty:isExperiencedBy
	a owl:ObjectProperty ;
	rdfs:label "is experienced by" ;
	rdfs:isDefinedBy <https://spec.edmcouncil.org/fibo/ontology/FND/Parties/Parties/> ;
	owl:inverseOf fibo-fnd-pty-pty:experiences ;
	owl:propertyChainAxiom (
		fibo-fnd-pty-pty:hasUndergoer
		fibo-fnd-pty-rl:isPlayedBy
	) ;
	skos:definition "relates a situation to something that is directly involved in or affected by it" ;
	.

fibo-fnd-pty-pty:playsActiveRoleIn
	a owl:ObjectProperty ;
	rdfs:label "plays active role in" ;
	rdfs:isDefinedBy <https://spec.edmcouncil.org/fibo/ontology/FND/Parties/Parties/> ;
	owl:propertyChainAxiom (
		fibo-fnd-pty-rl:playsRole
		fibo-fnd-pty-pty:actsIn
	) ;
	skos:definition "relates a person or organization to a situation that they are directly involved in" ;
	.

fibo-fnd-pty-pty:playsActiveRoleThatAffects
	a owl:ObjectProperty ;
	rdfs:label "plays active role that affects" ;
	rdfs:isDefinedBy <https://spec.edmcouncil.org/fibo/ontology/FND/Parties/Parties/> ;
	owl:inverseOf fibo-fnd-pty-pty:isDirectlyAffectedBy ;
	owl:propertyChainAxiom (
		fibo-fnd-pty-rl:playsRole
		fibo-fnd-pty-pty:actsIn
		fibo-fnd-pty-pty:hasUndergoer
	) ;
	skos:definition "relates a person or organization to an undergoer they have an impact on under the circumstances" ;
	.

fibo-fnd-pty-pty:playsActiveRoleThatDirectlyAffects
	a owl:ObjectProperty ;
	rdfs:label "plays active role that directly affects" ;
	rdfs:isDefinedBy <https://spec.edmcouncil.org/fibo/ontology/FND/Parties/Parties/> ;
	owl:inverseOf fibo-fnd-pty-pty:experiencesDirectly ;
	owl:propertyChainAxiom (
		fibo-fnd-pty-rl:playsRole
		fibo-fnd-pty-pty:actsIn
		fibo-fnd-pty-pty:hasUndergoer
		fibo-fnd-pty-rl:isPlayedBy
	) ;
	skos:definition "relates a person or organization to something they have a direct impact on under the circumstances" ;
	.

fibo-fnd-pty-pty:undergoes
	a owl:ObjectProperty ;
	rdfs:label "undergoes" ;
	rdfs:domain fibo-fnd-pty-pty:Undergoer ;
	rdfs:isDefinedBy <https://spec.edmcouncil.org/fibo/ontology/FND/Parties/Parties/> ;
	rdfs:range fibo-fnd-pty-pty:Situation ;
	owl:inverseOf fibo-fnd-pty-pty:hasUndergoer ;
	skos:definition "indicates a situation that the undergoer experiences" ;
	.

fibo-fnd-rel-rel:holds
	a owl:ObjectProperty ;
	rdfs:subPropertyOf fibo-fnd-pty-pty:directlyAffects ;
	.

fibo-fnd-rel-rel:isHeldBy
	a owl:ObjectProperty ;
	rdfs:subPropertyOf fibo-fnd-pty-pty:experiencesWith ;
	.

cmns-cxtdsg:ContextualName
	a owl:Class ;
	rdfs:subClassOf
		cmns-dsg:Name ,
		[
			a owl:Restriction ;
			owl:onProperty cmns-dsg:isNameOf ;
			owl:onClass fibo-fnd-pty-pty:IndependentParty ;
			owl:minQualifiedCardinality "0"^^xsd:nonNegativeInteger ;
		]
		;
	.

